\startcomponent *

\product  prd-analysis


\startchapter [title={Giuseppe Da Prato}]
	
	\startproposition [title={Proposition 1.2 in the book}, reference=prp:1d-Gaussian-measure]
		Let \m{a âˆˆ â„}, \m{Î» > 0}, and \m{Î¼ = N_{a, Q}}. Then
		\startitemize [i, joinedup]
			\item[1d-mean]  \m{âˆ«_â„ x N_{a, Î»}(\d x) = a},
			\item[1d-cov]  \m{âˆ«_â„ (x - a)^2 N_{a, Î»}(\d x) = Î»}, and
			\item[1d-Fourier]  \m{\widehat{N_{a, Î»}}(h) := âˆ«_â„ e^{ğš¤ h x} N_{a, Î»}(\d x) = e^{ğš¤ a h - \frac12 Î» h^2}}, \m{h âˆˆ â„}.
		\stopitemize
	\stopproposition

	\startproof
		\startitemize [i]
			\item  \m{âˆ«_â„ x N_{a, Î»}(\d x) = a},
			\item  \m{âˆ«_â„ (x - a)^2 N_{a, Î»}(\d x) = Î»}, and
			\item  \m{\widehat{N_{a, Î»}}(h) := âˆ«_â„ e^{ğš¤ h x} N_{a, Î»}(\d x) = e^{ğš¤ a h - \frac12 Î» h^2}}, \m{h âˆˆ â„}.
		\stopitemize
	\stopproof


	\startproposition [title={Proposition 1.3 in the book}]
		Let \m{H â‰ƒ â„^d} \m{a âˆˆ H}, \m{Q âˆˆ L_+(H)}, and \m{Î¼ = N_{a, Q}}. Then
		\startitemize [i, joinedup]
			\item[fd-mean]  \m{âˆ«_H x N_{a, Q}(\d x) = a},
			\item[fd-cov]  \m{âˆ«_H \inn[y, x - a] \inn[z, x - a] N_{a, Q}(\d x) = \inn[Qy, z]}, and
			\item[fd-Fourier]  \m{\widehat{N_{a, Q}}(h) := âˆ«_H e^{ğš¤ \inn[h, x]} N_{a, Q}(\d x) = e^{ğš¤ \inn[a, h] - \frac12 \inn[Qh, h]}}, \m{h âˆˆ H}.
		\stopitemize
 	\stopproposition

	\startproof
		All indices vary from \m{1} to \m{d}.
		\startitemize [i]

			\item  \m{âˆ«_H x N_{a, Q}(\d x) = a}.
				\startformula  \startalign[n=3]
					\NC  âˆ«_H x N_{a, Q}(\d x)  =  \NC  âˆ«_H x â¨‰_j N_{a_j, Î»_j} \brnd[â¨‰_i \d x_i]  \NR
					\NC  =  \NC  âˆ«_H âˆ‘_k(x_k e_k) âˆ_j N_{a_j, Î»_j}(\d x_j)  \NC  [\text{Fubini}]  \NR
					\NC  =  \NC  âˆ‘_k \brnd[âˆ«_â„ â‹¯ âˆ«_â„ x_k âˆ_j N_{a_j, Î»_j}(\d x_j)] e_k  \qquad  \NC  [\text{Fubini}]  \NR
					\NC  =  \NC  âˆ‘_k âˆ«_â„ x_k N_{a_k, Î»_k}(\d x_k) e_k  \NC  \bsqr[âˆ«_â„ N_{a_j, Î»_j}(\d x_j) = 1 \ âˆ€j]  \NR
					\NC  =  \NC  âˆ‘_k a_k e_k  \quad  =  a .  \NC  [\text{Proposition \in[prp:1d-Gaussian-measure](\in[1d-mean])}]  \NR
				\stopalign  \stopformula

			\item  \m{âˆ«_H \inn[y, x - a] \inn[z, x - a] N_{a, Q}(\d x) = \inn[Qy, z]}.
				\startformula  \startalign
					\NC     \NC  âˆ«_H \inn[y, x - a] \inn[z, x - a] N_{a, Q}(\d x)  \NR
					\NC  =  \NC  âˆ«_H âˆ‘_k y_k (x_k - a_k) âˆ‘_l z_l (x_l - a_l) âˆ_j N_{a_j, Î»_j}(\d x_j)  \NR
					\NC  =  \NC  âˆ‘_k âˆ‘_l y_k z_l âˆ«_H (x_k - a_k) (x_l - a_l) âˆ_j N_{a_j, Î»_j}(\d x_j)  \NR
					\NC  =  \NC  âˆ‘_k y_k z_k âˆ«_H (x_k - a_k)^2 âˆ_j N_{a_j, Î»_j}(\d x_j)  +  âˆ‘_{i â‰  j} y_k z_l âˆ«_H (x_k - a_k) (x_l - a_l) âˆ_j N_{a_j, Î»_j}(\d x_j)  \NR
					\NC  =  \NC  âˆ‘_k y_k z_k âˆ«_â„ (x_k - a_k)^2 N_{a_k, Î»_k}(\d x_k)  +  âˆ‘_{i â‰  j} y_k z_l âˆ«_â„ (x_k - a_k) N_{a_k, Î»_k} (\d x_k) âˆ«_â„ (x_l - a_l) N_{a_l, Î»_l}(\d x_l)  \NR
					\NC  =  \NC  âˆ‘_k y_k z_k Î»_k  \quad = \inn[Qy, z] .  \qquad  [\text{Proposition \in[prp:1d-Gaussian-measure](\in[1d-cov])}]  \NR
				\stopalign  \stopformula

			\item  \m{\widehat{N_{a, Q}}(h) := âˆ«_H e^{ğš¤ \inn[h, x]} N_{a, Q}(\d x) = e^{ğš¤ \inn[a, h] - \frac12 \inn[Qh, h]}}, \m{h âˆˆ H}.
				\startformula  \startalign[n=3]
					\NC  \widehat{N_{a, Q}}(h)  =  \NC  âˆ«_H e^{ğš¤ \inn[h, x]} N_{a, Q}(\d x)  \NR
					\NC  =  \NC  âˆ«_H e^{ğš¤ âˆ‘_k h_k x_k} âˆ_j N_{a_j, Î»_j}(\d x_j)  \NR
					\NC  =  \NC  âˆ«_H âˆ_k e^{ğš¤ h_k x_k} âˆ_j N_{a_j, Î»_j}(\d x_j)  \NR
					\NC  =  \NC  âˆ_k âˆ«_H e^{ğš¤ h_k x_k} N_{a_k, Î»_k}(\d x_k)  \NC  [\text{\comment{Why? This is false in general!}}]  \NR
					\NC  =  \NC  âˆ_k e^{ğš¤ a_k h_k - \frac12 Î»_k h_k^2}  \qquad  \NC  [\text{Proposition \in[prp:1d-Gaussian-measure](\in[1d-Fourier])}]  \NR
					\NC  =  \NC  e^{ğš¤ âˆ‘_k a_k h_k - \frac12 âˆ‘_k Î»_k h_k h_k}  \NR
					\NC  =  \NC  e^{ğš¤ \inn[a, h] - \frac12 \inn[Qh, h]} .  \NR
				\stopalign  \stopformula
		\stopitemize
	\stopproof

\stopchapter


\startchapter [title={Abstract Wiener spaces}, reference=chp:abstract-Wiener-spaces]

\stopchapter


\startchapter [title={White noise distribution theory}, reference=chp:white-noise-distribution-theory]

	\startsection [title={Characterization theorem}]

		Importance and history.

		In the following, \m{F} is defined on \m{S_â„‚}, and \m{F(z Î¾ + Î·)} is entire \m{âˆ€ z âˆˆ â„‚}.

		\startformula \startalign [
			n=9,
			align={middle, middle, middle, middle, middle, middle, middle, middle, middle}]
			\NC  (S)_Î²  \NC âŠ‚ \NC  (S)  \NC âŠ‚ \NC  (L^2)  \NC âŠ‚ \NC  (S)^*  \NC âŠ‚ \NC  (S)_Î²^*  \NR
			\NC  \NC \NC  S  \NC âŠ‚ \NC  L^2  \NC âŠ‚ \NC  S'  \NC \NC  \NR
		\stopalign \stopformula

	\stopsection

\stopchapter

\stopcomponent
