\startexercises [title={\getvariable{document}{author}  \hfill  \getvariable{document}{course}: HW1  \hfill  2019-09-10}]
	
	\startexercise [title={Notes, 1.8}]
		For any sets \m{A} and \m{B}, we have \m{A ∩ B ⊆ A}.
	\stopexercise
	\startsolution
		Let \m{x ∈ A ∩ B} be arbitrary. This means \m{x ∈ A} and \m{x ∈ B}. Therefore \m{x ∈ A}. Since every element in \m{A ∩ B} is also an element of \m{A}, we have \m{A ∩ B ⊆ A}.
	\stopsolution

	\startexercise [title={Notes, 1.10}]
		For any set \m{A}, we have \m{A ∩ ∅ = ∅}.
	\stopexercise
	\startsolution
		\bold{(\m{⊆})}  \qquad
		Let \m{x ∈ A ∩ ∅} be arbitrary. This means \m{x ∈ A} and \m{x ∈ ∅}. But there does not exist \m{x ∈ ∅}. Therefore, the statement is vacuously true.

		\bold{(\m{⊇})}  \qquad
		Now, let \m{x ∈ ∅} be arbitrary. Again, since there does not exist \m{x ∈ ∅}, the statement vacuously true.
	\stopsolution

	\startexercise [title={Notes, 1.13}]
		For any sets \m{A} and \m{B}, if \m{A ⊆ B}, then \m{A ∪ B = B}.
	\stopexercise
	\startsolution
		\bold{(\m{⊆})}  \qquad
		Let \m{x ∈ A ∪ B} be arbitrary. This means \m{x ∈ A} or \m{x ∈ B}. If \m{x ∈ A}, then by the condition \m{A ⊆ B}, we obtain \m{x ∈ B}. Therefore, in either case, \m{x ∈ B}.

		\bold{(\m{⊇})}  \qquad
		Let \m{x ∈ B} be arbitrary. Therefore, \m{x ∈ A} or \m{x ∈ B}. Hence \m{x ∈ A ∪ B}.
	\stopsolution

\stopexercises


\startexercises [title={\getvariable{document}{author}  \hfill  \getvariable{document}{course}: HW2  \hfill  2019-09-24}]

	\emph{Note:} We shall say that a truth assigment \m{v} satisfies \m{Σ} iff it satisfies every member of \m{Σ}.
	
	% \startexercise [title={\cite[short][EndertonLogic2001], 1.2.1}]
	\startexercise [title={Enderton, 1.2.1}]
		Show that neither of the following two formulas tautologically implies the other:
		\startformula  \startalign[align={right, left}]
			\NC  α =  \NC  (A ↔ (B ↔ C))  \NR
			\NC  β =  \NC  ((A ∧ (B ∧ C)) ∨ ((¬ A) ∧ ((¬ B) ∧ (¬ C))))  \NR
		\stopalign  \stopformula
	\stopexercise
	\startsolution
		We have to show that \m{α ⊭ β} and \m{β ⊭ α}.

		\bold{(\m{α ⊭ β})}  \qquad
		For this, it suffices to produce a truth assignment \m{v} such that \m{\bar{v}(α) = ⊤} and \m{\bar{v}(β) = ⊥}.

		Consider \m{v} such that \m{v(A) = v(B) = ⊥} and \m{v(C) = ⊤}. Under \m{\bar{v}}, we get exactly what is required as is shown in the computations below. (Here the truth assignments by \m{\bar{v}} is denoted under each symbol.)
		\startformula  \startalign[n=6, align={left, right, middle, right, middle, left}]
			\NC  α =  \NC  (A  \NC  ↔  \NC  (B  \NC  ↔  \NC  C))  \NR
			\NC  ⊤    \NC   ⊥  \NC  ⊤  \NC   ⊥  \NC  ⊥  \NC  ⊤    \NR
		\stopalign  \stopformula
		\startformula  \startalign[n=15, align={left, right, middle, middle, middle, middle, middle, right, left, middle, right, left, middle, right, left}]
			\NC  β =  \NC  ((A  \NC  ∧  \NC  (B  \NC  ∧  \NC  C))  \NC  ∨  \NC  ((¬  \NC  A)  \NC  ∧  \NC  ((¬  \NC  B)  \NC  ∧  \NC  (¬  \NC  C))))  \NR
			\NC  ⊥    \NC    ⊥  \NC  ⊥  \NC      \NC     \NC       \NC  ⊥  \NC       \NC      \NC  ⊥  \NC       \NC      \NC  ⊥  \NC   ⊥  \NC  ⊤      \NR
		\stopalign  \stopformula

		\bold{(\m{β ⊭ α})}  \qquad
		Again, it suffices to produce \m{v} such that \m{\bar{v}(β) = ⊤} and \m{\bar{v}(α) = ⊥}.

		Consider \m{v} such that \m{v(A) = v(B) = v(C) = ⊥}. Under \m{\bar{v}}, we get exactly what is required as is shown in the computations below.
		\startformula  \startalign[n=15, align={left, right, middle, middle, middle, middle, middle, right, left, middle, right, left, middle, right, left}]
			\NC  β =  \NC  ((A  \NC  ∧  \NC  (B  \NC  ∧  \NC  C))  \NC  ∨  \NC  ((¬  \NC  A)  \NC  ∧  \NC  ((¬  \NC  B)  \NC  ∧  \NC  (¬  \NC  C))))  \NR
			\NC  ⊤ =  \NC       \NC     \NC      \NC     \NC       \NC  ⊤  \NC    ⊤  \NC  ⊥   \NC  ⊤  \NC    ⊤  \NC  ⊥   \NC  ⊤  \NC   ⊤  \NC  ⊥      \NR
		\stopalign  \stopformula
		\startformula  \startalign[n=6, align={left, right, middle, right, middle, left}]
			\NC  α =  \NC  (A  \NC  ↔  \NC  (B  \NC  ↔  \NC  C))  \NR
			\NC  ⊥ =  \NC   ⊥  \NC  ⊥  \NC   ⊥  \NC  ⊤  \NC  ⊥    \NR
		\stopalign  \stopformula
	\stopsolution

	\page
	% \startexercise [title={\cite[short][EndertonLogic2001], 1.2.4 (a)}]
	\startexercise [title={Enderton, 1.2.4(a)}]
		Show that \m{Σ ∪ \bcrl[α] ⊨ β} iff \m{Σ ⊨ (α → β)}.
	\stopexercise
	\startsolution
		We show each direction separately.

		\bold{(\m{⟹})}  \qquad
		% We show this by contrapositive. Suppose \m{Σ ⊭ (α → β)}. Since
		We suppose \m{Σ ∪ \bcrl[α] ⊨ β}. Let \m{v} be an arbitrary truth assignment that satisfies \m{Σ}. We have to show that \m{v} satisfies \m{(α → β)}. We have two cases.
		\startitemize [i, joinedup]
			\item  \m{\bar{v}(α) = ⊤}: In this case, from the supposition, we get \m{\bar{v}(β) = ⊤}. So \m{\bar{v}(α → β) = ⊤}.
			\item  \m{\bar{v}(α) = ⊥}: In this case, \m{\bar{v}(α → β) = ⊤} since the antecedent is \m{⊥}.
		\stopitemize
		Since \m{v} was arbitrary, we have \m{Σ ⊨ (α → β)}.

		\bold{(\m{⟸})}  \qquad
		We suppose \m{Σ ⊨ (α → β)}. Let \m{v} be an arbitrary truth assignment that satisfies \m{Σ ∪ \bcrl[α]}. We have to show that \m{v} satisfies \m{β}. Since \m{v} satisfies \m{Σ ∪ \bcrl[α]}, it satisfies \m{Σ}. Therefore, by our supposition, \m{v} satisfies \m{(α → β)}. Now, since \m{v} satisfies \m{α}, it can only be that \m{v} satisfies \m{β}, since the only other way the material implication can be satisfied is when \m{v} does not satisfies \m{α}. This proves our claim.
	\stopsolution

	% \startexercise [title={\cite[short][EndertonLogic2001], 1.2.5}]
	\startexercise [title={Enderton, 1.2.5}]
		Prove or refute each of the following assertions:
		\startitemize [a, joinedup]

			\item  If either \m{Σ ⊨ α} or \m{Σ ⊨ β}, then \m{Σ ⊨ (α ∨ β)}.

				\startsolution
					(\bold{⊤})  \qquad
					There are two cases: \m{Σ ⊨ α} and \m{Σ ⊨ β}. Without loss of generality, we can assume that \m{Σ ⊨ α}, as the argument for other case is exactly the same. This means any arbitrary truth assignment \m{v} satisfying \m{Σ} also satisfies \m{α}. This implies \m{\bar{v}(α ∨ β) = ⊤} by the definition of extension of \m{\bar{v}} for \m{∨}.
				\stopsolution

			\item  If \m{Σ ⊨ (α ∨ β)}, then either \m{Σ ⊨ α} or \m{Σ ⊨ β}.

				\startsolution
					(\bold{⊥})  \qquad
					We give a counterexample. Let \m{α} be a sentence symbol and \m{Σ = ∅}. Then it is always true that \m{⊨ (α ∨ (¬α))}. But it does not follow that \m{⊨ α} or \m{⊨ (¬α)}.

					For an explicit example, consider two truth assignments \m{v_1} and \m{v_2}, such that \m{v_1(α) = ⊤} and \m{v_2(α) = ⊥}. In this case, \m{⊨ α} is not true since \m{v_2} does not satisfy \m{α}, and \m{⊨ (¬α)} is not true since \m{v_1} does not satisfy \m{(¬α)}.
				\stopsolution
		\stopitemize
	\stopexercise

	\page
	% \startexercise [title={\cite[short][EndertonLogic2001], 1.2.6}]
	\startexercise [title={Enderton, 1.2.6}]
		\startitemize [a, joinedup]

			\item[uniqueness]  Show that if \m{v_1} and \m{v_2} are truth assignments which agree on all the sentence symbols in the wff \m{α}, then \m{\bar{v}_1(α)} = \m{\bar{v}_2(α)}.

				\startsolution
					
					Let \m{G} be the set of sentence symbols used in \m{α}, and let \m{B = \bcrl[ϕ \text{ wff}: \bar{v}_1(ϕ) = \bar{v}_2(ϕ)]}. All we need to show is that \m{α ∈ B}.

					Firstly, \m{G ⊆ B} since \m{v_1} and \m{v_2} agree on the sentence symbols used in \m{α}.

					Secondly, let \m{ϕ, ψ ∈ B} (arbitrary), so \m{v_1} and \m{v_2} agree on \m{ϕ} and \m{ψ}. Let \m{⊡ ∈ \bcrl[∧, ∨, →, ↔]}. Since conditions 1–5 on page 20–21 are the same for \m{\bar{v}_1} and \m{\bar{v}_2}, we have \m{\bar{v}_1(¬ ϕ) = \bar{v}_2(¬ ϕ)} and \m{\bar{v}_1(ϕ ⊡ ψ) = \bar{v}_2(ϕ ⊡ ψ)}. Hence \m{(¬ϕ), (ϕ ⊡ ψ) ∈ B}, that is, \m{B} is closed with respect to the formula building operations.

					Therefore, by the induction principle, \m{B} is the set of \emph{all} wffs generated by the formula building operations. So \m{α ∈ B}, and we are done.
				\stopsolution
			
			\item  Let \m{S} be a set of sentence symbols that includes those in \m{Σ} and \m{τ} (and possibly more). Show that \m{Σ ⊨ τ} iff every truth assignment for \m{S} which satisfies every member of \m{Σ} also satisfies \m{τ}.

				\startsolution
					In this part, we use \m{v} to denote truth assignments and \quotation{\m{v} on a set} means \m{v} is defined on that set. Let \m{G} be the set of sentence symbols used in \m{Σ} and \m{τ}. Clearly, \m{G ⊆ S}.

					We show each direction separately.

					\bold{(\m{⟹})}  \qquad
					From the definition of tautological implication,
					\startformula  \startalign[n=3]
						\NC     \NC  Σ ⊨ τ  \NR
						\NC  ⟺  \NC  (∀ v \text{ on } G) ((v \text{ satisfies } Σ) → (v \text{ satisfies } τ))  \NR
						\NC  ⟹  \NC  (∀ v \text{ on } S) ((v \text{ satisfies } Σ) → (v \text{ satisfies } τ))  \NC  \text{[Part (\in[uniqueness])]}  \NR
					\stopalign  \stopformula
					
					\bold{(\m{⟸})}  \qquad
					Since \m{Σ} and \m{τ} does not depend on any element of \m{S ∖ G}, restricting the definition of \m{v} from \m{S} to \m{G} will not change anything on \m{Σ} and \m{τ}. Therefore,
					\startformula  \startalign
						\NC     \NC  (∀ v \text{ on } S) ((v \text{ satisfies } Σ) → (v \text{ satisfies } τ))  \NR
						\NC  ⟹  \NC  (∀ v \text{ on } G) ((v \text{ satisfies } Σ) → (v \text{ satisfies } τ))  \NR
						\NC  ⟺  \NC  Σ ⊨ τ  \NR
					\stopalign  \stopformula
				  
				\stopsolution
		\stopitemize
	\stopexercise
\stopexercises


\startexercises [title={\getvariable{document}{author}  \hfill  \getvariable{document}{course}: Prelim  \hfill  2019-10-08}]

	\startexercise [title={Set Theory}]
		Prove the following. 10 points each.

		\emph{Note}: Let \m{A} and \m{B} are sets. In order to prove \m{A = B}, it is enough to show \m{A ⊆ B} and \m{A ⊇ B}. In each of the following problems, we show each inclusion separately.

		Moreover, to show \m{A ⊆ B}, it suffices to show that for \m{x} arbitrary, \m{x ∈ A ⟹ x ∈ B}.

		\startitemize [i]
			\item  If \m{A ⊆ B}, then \m{A ∩ B = A}.

				\startsolution
					\startitemize
						
						\sym{\bold{(⊆)}}  \qquad
							Let \m{x} be arbitrary. Then

							\m{x ∈ A ∩ B  \quad ⟺ \quad  x ∈ A \text{ and } x ∈ B  \quad ⟹ \quad  x ∈ A}.

						\sym{\bold{(⊇)}}  \qquad
							Let \m{x ∈ A} be arbitrary. Then by the hypothesis \m{x ∈ B} since \m{A ⊆ B}. Therefore, \m{x ∈ A} and \m{x ∈ B}, and thus \m{x ∈ A ∩ B}.
					\stopitemize
				\stopsolution

			\item  If \m{A ∩ B = ∅}, then \m{A ∖ B = A}.

				\startsolution
					\startitemize
						
						\sym{\bold{(⊆)}}  \qquad
							Let \m{x ∈ A ∖ B} be arbitrary. Then \m{x ∈ A} and \m{x ∉ B}. It is enough to show that \m{x ∈ A} implies \m{x ∉ B}. But must be true since if \m{x ∈ A} and \m{x ∈ B}, then \m{x ∈ A ∩ B = ∅}, which is absurd.

						\sym{\bold{(⊇)}}  \qquad
							Let \m{x ∈ A} be arbitrary. Now, either \m{x ∈ B} or \m{x ∉ B}. If \m{x ∈ B}, then \m{x ∈ A ∩ B} since \m{x ∈ A} by hypothesis. But this is an impossibility since \m{A ∩ B = ∅}. Therefore, it must be that \m{x ∉ B}. So \m{x ∈ A ∖ B}.
					\stopitemize
				\stopsolution
				
			\item  \m{A ∩ (B ∪ C) = (A ∩ B) ∪ (A ∩ C)}.

				\startsolution
					\startitemize
						
						\sym{\bold{(⊆)}}  \qquad
							Let \m{x ∈ A ∩ (B ∪ C)} be arbitrary. Then \m{x ∈ A} and \m{x ∈ B ∪ C}. Note that \m{x ∈ B ∪ C} means \m{x ∈ B} or \m{x ∈ C}.
							Now, either \m{x ∈ B} or \m{x ∉ B}, so have two cases.
							\startitemize [1]
								\item  (\m{x ∈ B})  \qquad
									In this case, \m{x ∈ A} and \m{x ∈ B}, so \m{x ∈ A ∩ B}. Therefore \m{x ∈ A ∩ B} or \m{x ∈ A ∩ C}. Hence \m{x ∈ (A ∩ B) ∪ (A ∩ C)}.
								\item  (\m{x ∉ B})  \qquad
									Since \m{x ∈ B} or \m{x ∈ C}, and \m{x ∉ B}, it is necessary that \m{x ∈ C}. Therefore we get the exact same result by interchanging the roles of \m{B} and \m{C} in the previous case.
							\stopitemize

						\sym{\bold{(⊇)}}  \qquad
							Let \m{x ∈ (A ∩ B) ∪ (A ∩ C)} be arbitrary. This means \m{x ∈ A ∩ B} or \m{x ∈ A ∩ C}. As above, we have two cases, either \m{x ∈ A ∩ B} or \m{x ∉ A ∩ B}.
							\startitemize [1]
								\item  (\m{x ∈ A ∩ B})  \qquad
									In this case, \m{x ∈ A} and \m{x ∈ B}. Now, so \m{x ∈ B} implies \m{x ∈ B} or \m{x ∈ C}, that is, \m{x ∈ B ∪ C}. Therefore \m{x ∈ A ∩ (B ∪ C)}.
								\item  (\m{x ∉ A ∩ B})  \qquad
									Again, since \m{x ∈ A ∩ B} or \m{x ∉ A ∩ B}, and \m{x ∉ A ∩ B}, it is necessary that \m{x ∈ A ∩ C}. Therefore we get the exact same result by interchanging the roles of \m{B} and \m{C} in the previous case.
							\stopitemize
					\stopitemize
				\stopsolution				
		\stopitemize
	\stopexercise

	
	\startexercise [title={Construction}]
		10 points each.
		\startitemize [i]

			\item  Write down a construction sequence for \m{((¬((¬A_1) ∨ A_4)) ∧ ((A_1 → A_3) ↔ A_7))}.

				\startsolution
					\m{⟨A_1,\ A_3,\ A_4,\ A_7,\ (¬A_1),\ ((¬A_1) ∨ A_4),\ (¬((¬A_1) ∨ A_4)),\ (A_1 → A_3),\ ((A_1 → A_3) ↔ A_7),\ ((¬((¬A_1) ∨ A_4)) ∧ ((A_1 → A_3) ↔ A_7))⟩}.
				\stopsolution
				
			\item  Write down a construction tree for \m{(((¬(¬ A_2)) ∧ A_5) → ((A_5 ∨ (¬A_2)) → A_5))}.

				\startsolution
					\starttikzpicture [
						baseline,    % Sets the baseline to the baseline of the text.
						level distance=2em,
						every node/.style={fill=\getvariable{document}{color-headings}!10, circle, inner sep=1pt},
						level 1/.style={sibling distance=8em},
						level 2/.style={sibling distance=4em},
						level 3/.style={sibling distance=2em}]
						
						\node {→} % root
						child { node {∧}
							child { node {¬}
								child { node {¬}
									child { node {\m{A_2}} }
								}
							}
							child { node {\m{A_5}} }
						}
						child { node {→}
							child { node {∨}
								child { node {\m{A_5}} }
								child { node {¬}
									child { node {\m{A_2}} }
								}
							}
							child { node {\m{A_5}} }
						};
					\stoptikzpicture				
				\stopsolution
		\stopitemize
	\stopexercise

	
	\page
	\startexercise [title={Truth Assignments}]
		\startitemize [i]

			\item  Let \m{S} be the set of all sentence symbols, and assume that \m{v : S → \bcrl[F, T]} is a truth assignment. Show there is at most one extension \m{v} meeting conditions 0–5 on pp. 20–21.

				(Hint: Show that if \m{v_1} and \m{v_2} are such extensions, then \m{\bar{v}_1(α) = \bar{v}_2(α)} for every wff \m{α}. Use the induction principle.)  20 points.

				\startsolution
					We show this via induction on the complexity of any arbitrary wff \m{α}.
					\startitemize [1]
						
						\item  \bold{(Base case)}  \qquad
							Assume \m{α} be a sentence symbol. Then \m{\bar{v}_1(α) = v(α) = \bar{v}_2(α)} since \m{\bar{v}_1} and \m{\bar{v}_2} are both extensions of \m{v}.

						\item  \bold{(Induction step)}  \qquad
							We assume that the result holds for all wffs less complex than \m{α} (induction hypothesis). Now, we show that the result holds under all the formula building operations.
							\startitemize
								\sym{(¬)}  \qquad
									Assume \m{α = (¬β)} for some wff \m{β}. Then
									\startformula  \startalign[n=4, align={left, right, left, left}]
										\NC     \NC  \bar{v}_1( α)  \NC  =  ⊤  \NR
										\NC  ⟺  \NC  \bar{v}_1(¬β)  \NC  =  ⊤  \NC  \qquad  [\text{Def of \m{α}}]  \NR
										\NC  ⟺  \NC  \bar{v}_1( β)  \NC  =  ⊥  \NC  \qquad  [\text{Def of \m{\bar{v}} under \m{¬}}]  \NR
										\NC  ⟺  \NC  \bar{v}_2( β)  \NC  =  ⊥  \NC  \qquad  [\text{Induction hypothesis}]  \NR
										\NC  ⟺  \NC  \bar{v}_2(¬β)  \NC  =  ⊤  \NC  \qquad  [\text{Def of \m{\bar{v}} under \m{¬}}]  \NR
										\NC  ⟺  \NC  \bar{v}_2( α)  \NC  =  ⊤  \NC  \qquad  [\text{Def of \m{α}}]  \NR
									\stopalign  \stopformula
								\sym{(∧)}  \qquad
									Assume \m{α = (β ∧ γ)} for some wffs \m{β, γ}. Then
									\startformula  \startalign[n=4, align={right, right, left, left}]
										\NC     \NC  \bar{v}_1(α)  \NC  =  ⊤  \NR
										\NC  ⟺  \NC  \bar{v}_1(β ∧ γ)  \NC  =  ⊤  \NC  \qquad  [\text{Def of \m{α}}]  \NR
										\NC  ⟺  \NC   \bar{v}_1(β) = ⊤  \NC  \text{ and }  \bar{v}_1(γ) = ⊤  \NC  \qquad  [\text{Def of \m{\bar{v}} under \m{∧}}]  \NR
										\NC  ⟺  \NC   \bar{v}_2(β) = ⊤  \NC  \text{ and }  \bar{v}_2(γ) = ⊤  \NC  \qquad  [\text{Induction hypothesis}]  \NR
										\NC  ⟺  \NC  \bar{v}_2(β ∧ γ)  \NC  =  ⊤  \NC  \qquad  [\text{Def of \m{\bar{v}} under \m{∧}}]  \NR
										\NC  ⟺  \NC   \bar{v}_2(α)  \NC  =  ⊤  \NC  \qquad  [\text{Def of \m{α}}]  \NR
									\stopalign  \stopformula
								\sym{(∨)}  \qquad
									Assume \m{α = (β ∨ γ)} for some wffs \m{β, γ}. Then
									\startformula  \startalign[n=4, align={right, right, left, left}]
										\NC     \NC  \bar{v}_1(α)  \NC  =  ⊤  \NR
										\NC  ⟺  \NC  \bar{v}_1(β ∨ γ)  \NC  =  ⊤  \NC  \qquad  [\text{Def of \m{α}}]  \NR
										\NC  ⟺  \NC   \bar{v}_1(β) = ⊤  \NC  \text{ or }  \bar{v}_1(γ) = ⊤  \NC  \qquad  [\text{Def of \m{\bar{v}} under \m{∨}}]  \NR
										\NC  ⟺  \NC   \bar{v}_2(β) = ⊤  \NC  \text{ or }  \bar{v}_2(γ) = ⊤  \NC  \qquad  [\text{Induction hypothesis}]  \NR
										\NC  ⟺  \NC  \bar{v}_2(β ∨ γ)  \NC  =  ⊤  \NC  \qquad  [\text{Def of \m{\bar{v}} under \m{∨}}]  \NR
										\NC  ⟺  \NC   \bar{v}_2(α)  \NC  =  ⊤  \NC  \qquad  [\text{Def of \m{α}}]  \NR
									\stopalign  \stopformula
								\sym{(→)}  \qquad
									Assume \m{α = (β → γ)} for some wffs \m{β, γ}. Then
									\startformula  \startalign[n=4, align={right, right, left, left}]
										\NC     \NC  \bar{v}_1(α)  \NC  =  ⊤  \NR
										\NC  ⟺  \NC  \bar{v}_1(β → γ)  \NC  =  ⊤  \NC  \qquad  [\text{Def of \m{α}}]  \NR
										\NC  ⟺  \NC   \bar{v}_1(β) = ⊥  \NC  \text{ or }  \bar{v}_1(γ) = ⊤  \NC  \qquad  [\text{Def of \m{\bar{v}} under \m{→}}]  \NR
										\NC  ⟺  \NC   \bar{v}_2(β) = ⊥  \NC  \text{ or }  \bar{v}_2(γ) = ⊤  \NC  \qquad  [\text{Induction hypothesis}]  \NR
										\NC  ⟺  \NC  \bar{v}_2(β → γ)  \NC  =  ⊤  \NC  \qquad  [\text{Def of \m{\bar{v}} under \m{→}}]  \NR
										\NC  ⟺  \NC   \bar{v}_2(α)  \NC  =  ⊤  \NC  \qquad  [\text{Def of \m{α}}]  \NR
									\stopalign  \stopformula
								\sym{(↔)}  \qquad
									Assume \m{α = (β ↔ γ)} for some wffs \m{β, γ}. Then
									\startformula  \startalign[n=4, align={right, right, left, left}]
										\NC     \NC  \bar{v}_1(α)  \NC  =  ⊤  \NR
										\NC  ⟺  \NC  \bar{v}_1(β ↔ γ)  \NC  =  ⊤  \NC  \qquad  [\text{Def of \m{α}}]  \NR
										\NC  ⟺  \NC  \bar{v}_1(β)  \NC  =  \bar{v}_1(γ)  \NC  \qquad  [\text{Def of \m{\bar{v}} under \m{↔}}]  \NR
										\NC  ⟺  \NC  \bar{v}_2(β)  \NC  =  \bar{v}_2(γ)  \NC  \qquad  [\text{Induction hypothesis}]  \NR
										\NC  ⟺  \NC  \bar{v}_2(β ↔ γ)  \NC  =  ⊤  \NC  \qquad  [\text{Def of \m{\bar{v}} under \m{↔}}]  \NR
										\NC  ⟺  \NC  \bar{v}_2(α)  \NC  =  ⊤  \NC  \qquad  [\text{Def of \m{α}}]  \NR
									\stopalign  \stopformula
							\stopitemize
					\stopitemize
					Therefore, the induction step holds under all the formula building operations. By the method of induction, \m{\bar{v}_1(α) = \bar{v}_2(α)} for every wff \m{α}, which proves the uniqueness of the extension.
				\stopsolution

			\item[satisfiability]  Show that for a set of wffs \m{Σ} and a wff \m{α}: \m{Σ ∪ \bcrl[¬¬α]} is satisfiable ⟺ \m{Σ ∪ \bcrl[α]} is satisfiable. 10 points.

				\startsolution
					First, note that for any wff \m{α} and truth assignment \m{v},
					\startformula
						\bar{v}(α) = ⊤  \quad ⟺ \quad  \bar{v}(¬α) = ⊥  \quad ⟺ \quad  \bar{v}(¬¬α) = ⊤ .
					\stopformula
					Therefore, we have the following (\m{v} always represents a truth assignment):
					\startitemize [joinedup]
						\sym{ }  \qquad  \m{Σ ∪ \bcrl[α]} is satisfiable.
						\sym{⟺}  \qquad  \m{∃v} such that \m{v} satisfies \m{Σ} and \m{\bar{v}(α) = ⊤}.
						\sym{⟺}  \qquad  \m{∃v} such that \m{v} satisfies \m{Σ} and \m{\bar{v}(¬α) = ⊥}.
						\sym{⟺}  \qquad  \m{∃v} such that \m{v} satisfies \m{Σ} and \m{\bar{v}(¬¬α) = ⊤}.
						\sym{⟺}  \qquad  \m{Σ ∪ \bcrl[¬¬α]} is satisfiable.
					\stopitemize
				\stopsolution
		\stopitemize
	\stopexercise


	\page
	\startexercise [title={Compactness}]

		Recall the Compactness Theorem: A set of wffs is satisfiable iff it is finitely satisfiable.
	
		Recall Corollary 17A: If \m{Σ ⊨ τ}, then \m{Σ_0 ⊨ τ} for some finite \m{Σ_0 ⊆ Σ}.
	
		Prove that they are equivalent, i.e., prove that the Compactness Theorem holds iff Corollary 17A holds.

		(Hint: Use the fact that \m{Γ ⊨ σ} iff \m{Γ ∪ \bcrl[¬σ]} is unsatisfiable and 3.3.\in[satisfiability] above.) 20 points.
	\stopexercise

	
	\startexercise [title={Substitution}]
		Let \m{α_1, α_2, …} be a sequence of wffs. For each wff \m{ϕ} and \m{n ∈ ℕ}, let \m{ϕ^∗} be the result of replacing the sentence symbol \m{A_n} in \m{ϕ} by the wff \m{α_n}. Suppose that \m{v} is a truth assignment for the set of all sentence symbols and that \m{u} is a truth assignment defined by \m{u(A_n) = \bar{v}(α_n)}. Show that \m{\bar{u}(ϕ) = \bar{v}(ϕ^∗)}. 

		(Hint: Use the induction principle.)  20 points
	\stopexercise

	\startsolution
		We show this via induction on the complexity of any arbitrary wff \m{ϕ}.
		\startitemize [1]
			
			\item  \bold{(Base case)}  \qquad
				Assume \m{ϕ = A_n} for some \m{n ∈ ℕ}, so \m{ϕ^* = α_n}. Now \m{\bar{u}(ϕ) = \bar{u}(A_n) = u(A_n) = \bar{v}(α_n) = \bar{v}(ϕ^∗)}, so the result holds when \m{ϕ} is a sentence symbol.

			\item  \bold{(Induction step)}  \qquad
				We assume that the result holds for all wffs less complex than \m{ϕ} (induction hypothesis). Now, we show that the result holds under all the formula building operations.
				\startitemize
					\sym{(¬)}  \qquad
						Assume \m{ϕ = (¬ψ)} for some wff \m{ψ}, so \m{ϕ^* = (¬ψ^*)}. Then
						\startformula  \startalign[n=4, align={left, right, left, left}]
							\NC     \NC  \bar{u}( ϕ  )  \NC  =  ⊤  \NR
							\NC  ⟺  \NC  \bar{u}(¬ψ  )  \NC  =  ⊤  \NC  \qquad  [\text{Def of \m{ϕ}}]  \NR
							\NC  ⟺  \NC  \bar{u}( ψ  )  \NC  =  ⊥  \NC  \qquad  [\text{Def of \m{\bar{u}} under \m{¬}}]  \NR
							\NC  ⟺  \NC  \bar{v}( ψ^*)  \NC  =  ⊥  \NC  \qquad  [\text{Induction hypothesis}]  \NR
							\NC  ⟺  \NC  \bar{v}(¬ψ^*)  \NC  =  ⊤  \NC  \qquad  [\text{Def of \m{\bar{v}} under \m{¬}}]  \NR
							\NC  ⟺  \NC  \bar{v}( ϕ^*)  \NC  =  ⊤  \NC  \qquad  [\text{Def of \m{ϕ^*}}]  \NR
						\stopalign  \stopformula
					\sym{(∧)}  \qquad
						Assume \m{ϕ = (ψ ∧ θ)} for some wffs \m{ψ, θ}, so \m{ϕ^* = (ψ^* ∧ θ^*)}. Then
						\startformula  \startalign[n=4, align={right, right, left, left}]
							\NC     \NC  \bar{u}(ϕ)  \NC  =  ⊤  \NR
							\NC  ⟺  \NC  \bar{u}(ψ ∧ θ)  \NC  =  ⊤  \NC  \qquad  [\text{Def of \m{ϕ}}]  \NR
							\NC  ⟺  \NC   \bar{u}(ψ) = ⊤  \NC  \text{ and }  \bar{u}(θ) = ⊤  \NC  \qquad  [\text{Def of \m{\bar{u}} under \m{∧}}]  \NR
							\NC  ⟺  \NC   \bar{v}(ψ^*) = ⊤  \NC  \text{ and }  \bar{v}(θ^*) = ⊤  \NC  \qquad  [\text{Induction hypothesis}]  \NR
							\NC  ⟺  \NC  \bar{v}(ψ^* ∧ θ^*)  \NC  =  ⊤  \NC  \qquad  [\text{Def of \m{\bar{v}} under \m{∧}}]  \NR
							\NC  ⟺  \NC   \bar{v}(ϕ^*)  \NC  =  ⊤  \NC  \qquad  [\text{Def of \m{ϕ^*}}]  \NR
						\stopalign  \stopformula
					\sym{(∨)}  \qquad
						Assume \m{ϕ = (ψ ∨ θ)} for some wffs \m{ψ, θ}, so \m{ϕ^* = (ψ^* ∨ θ^*)}. Then
						\startformula  \startalign[n=4, align={right, right, left, left}]
							\NC     \NC  \bar{u}(ϕ)  \NC  =  ⊤  \NR
							\NC  ⟺  \NC  \bar{u}(ψ ∨ θ)  \NC  =  ⊤  \NC  \qquad  [\text{Def of \m{ϕ}}]  \NR
							\NC  ⟺  \NC   \bar{u}(ψ) = ⊤  \NC  \text{ or }  \bar{u}(θ) = ⊤  \NC  \qquad  [\text{Def of \m{\bar{u}} under \m{∨}}]  \NR
							\NC  ⟺  \NC   \bar{v}(ψ^*) = ⊤  \NC  \text{ or }  \bar{v}(θ^*) = ⊤  \NC  \qquad  [\text{Induction hypothesis}]  \NR
							\NC  ⟺  \NC  \bar{v}(ψ^* ∨ θ^*)  \NC  =  ⊤  \NC  \qquad  [\text{Def of \m{\bar{v}} under \m{∨}}]  \NR
							\NC  ⟺  \NC   \bar{v}(ϕ^*)  \NC  =  ⊤  \NC  \qquad  [\text{Def of \m{ϕ^*}}]  \NR
						\stopalign  \stopformula
					\sym{(→)}  \qquad
						Assume \m{ϕ = (ψ → θ)} for some wffs \m{ψ, θ}, so \m{ϕ^* = (ψ^* → θ^*)}. Then
						\startformula  \startalign[n=4, align={right, right, left, left}]
							\NC     \NC  \bar{u}(ϕ)  \NC  =  ⊤  \NR
							\NC  ⟺  \NC  \bar{u}(ψ → θ)  \NC  =  ⊤  \NC  \qquad  [\text{Def of \m{ϕ}}]  \NR
							\NC  ⟺  \NC   \bar{u}(ψ) = ⊥  \NC  \text{ or }  \bar{u}(θ) = ⊤  \NC  \qquad  [\text{Def of \m{\bar{u}} under \m{→}}]  \NR
							\NC  ⟺  \NC   \bar{v}(ψ^*) = ⊥  \NC  \text{ or }  \bar{v}(θ^*) = ⊤  \NC  \qquad  [\text{Induction hypothesis}]  \NR
							\NC  ⟺  \NC  \bar{v}(ψ^* → θ^*)  \NC  =  ⊤  \NC  \qquad  [\text{Def of \m{\bar{v}} under \m{→}}]  \NR
							\NC  ⟺  \NC   \bar{v}(ϕ^*)  \NC  =  ⊤  \NC  \qquad  [\text{Def of \m{ϕ^*}}]  \NR
						\stopalign  \stopformula
					\sym{(↔)}  \qquad
						Assume \m{ϕ = (ψ ↔ θ)} for some wffs \m{ψ, θ}, so \m{ϕ^* = (ψ^* ↔ θ^*)}. Then
						\startformula  \startalign[n=4, align={right, right, left, left}]
							\NC     \NC  \bar{u}(ϕ)  \NC  =  ⊤  \NR
							\NC  ⟺  \NC  \bar{u}(ψ ↔ θ)  \NC  =  ⊤  \NC  \qquad  [\text{Def of \m{ϕ}}]  \NR
							\NC  ⟺  \NC  \bar{u}(ψ)  \NC  =  \bar{u}(θ)  \NC  \qquad  [\text{Def of \m{\bar{u}} under \m{↔}}]  \NR
							\NC  ⟺  \NC  \bar{v}(ψ^*)  \NC  =  \bar{v}(θ^*)  \NC  \qquad  [\text{Induction hypothesis}]  \NR
							\NC  ⟺  \NC  \bar{v}(ψ^* ↔ θ^*)  \NC  =  ⊤  \NC  \qquad  [\text{Def of \m{\bar{v}} under \m{↔}}]  \NR
							\NC  ⟺  \NC  \bar{v}(ϕ^*)  \NC  =  ⊤  \NC  \qquad  [\text{Def of \m{ϕ^*}}]  \NR
						\stopalign  \stopformula
				\stopitemize
		\stopitemize
		Therefore, the induction step holds under all the formula building operations. By the method of induction, \m{\bar{u}(ϕ) = \bar{v}(ϕ)} for every wff \m{ϕ}.
	\stopsolution

\stopexercises

% \startformula  \startalign

% \stopalign  \stopformula
