\startcomponent *

\product  prd-research


\startchapter [title={Friedlin-Wentzell theorem}, reference=chp:Friedlin-Wentzell-theorem]


\stopchapter


\startchapter [title={Friedlin-Wentzell theorem for anticipating initial condition with extension of filtration}, reference=chp:FW-anticipating-IC-extension-filtration]
	
	Our aim is to formulate a large deviations principle for an SDE with anticipating initial conditions. We start of with a very simple case
	\startformula
		X_t^ε = W_T + \sqrt{ε} ∫_0^t σ(X_t^ε) \d W_t ,
	\stopformula
	where \m{t ∈ [0, T]} for some \m{T < ∞}, and conditions on \m{σ} shall be imposed as necessary.

	We shall look at the method of enlargement of filtration by \cite[short][Itô1978]. We denote the enlarged filtration by \m{\tilde{ℱ}_t = ℱ_t ∨ σ(W_T)}. For \m{t ∈ [0, T]}, define the process \m{A_t = ∫_0^t \frac{W_T - W_u}{T - u} \d u}. Then \m{W_t = \tilde{W}_t + A_t}, where \m{\tilde{W}_⋅} is a Wiener process w.r.t. \m{\tilde{ℱ}_⋅}.

	For now, we shall bound \m{t ∈ [0, T_b]}, where \m{T_b ∈ [0, T)}.
	\comment{What happens when \m{t → T}?}

	Using this, we write our original SDE as
	\startformula
		X_t^ε = W_T + \sqrt{ε} ∫_0^t σ(X_t^ε) \d \tilde{W}_t + \sqrt{ε} ∫_0^t σ(X_t^ε) \frac{W_T - W_s}{T - s} \d s .
	\stopformula
	Let \m{Y_t^ε = \sqrt{ε} (W_T - W_t)}. Then \m{X_t^ε} is given by
	\startformula
		X_t^ε = W_T + \sqrt{ε} ∫_0^t σ(X_t^ε) \d \tilde{W}_t + ∫_0^t σ(X_t^ε) \frac{Y_s^ε}{T - s} \d s .
	\stopformula

	Moreover,
	\startformula  \startalign
		\NC  Y_t^ε  \NC  =  \sqrt{ε} W_T - \sqrt{ε} W_t  \NR
		\NC  \NC  =  \sqrt{ε} W_T - \sqrt{ε} \brnd[\tilde{W}_t + ∫_0^t \frac{W_T - W_s}{T - s} \d s]  \NR
		\NC  \NC  =  \sqrt{ε} W_T - \sqrt{ε} \tilde{W}_t - ∫_0^t \frac{Y_s^ε}{T - s} \d s  \NR
	\stopalign  \stopformula

	Therefore, we have the joint process
	\startformula
		\startrndmatrix
			X_t^ε  \NR  Y_t^ε  \NR
		\stoprndmatrix
		=
		\startrndmatrix
			1  \NR  \sqrt{ε}  \NR
		\stoprndmatrix
		W_T  +  \sqrt{ε} ∫_0^t
		\startrndmatrix
			σ(X_s^ε)  \NR  -1  \NR
		\stoprndmatrix
		\d \tilde{W}_s  +  ∫_0^t
		\startrndmatrix
			σ(X_s^ε)  \NR  -1  \NR
		\stoprndmatrix
		\frac{Y_s^ε}{T - s} \d s .
	\stopformula

	Firstly, we show that there is a unique solution to the above system of SDEs. For convinience, let \m{\tilde{σ}(x, y) = (σ(x), -1)} and \m{\tilde{b}(x, y) = \frac{y}{T - s} (σ(x), -1)}.
	\startproposition
		\m{\tilde{σ}} and \m{\tilde{b}} satisfy the linear growth and Lipshitz conditions.
	\stopproposition
	\startproof
		
	\stopproof

	Note that \m{Y_t^ε → 0} as \m{ε → 0}. Therefore, we expect
	\startformula
		\startrndmatrix
			X_t^ε - W_T  \NR  Y_t^ε  \NR
		\stoprndmatrix
		→
		\startrndmatrix
			0  \NR  0  \NR
		\stoprndmatrix
		\text{ as } ε → 0 .
	\stopformula

	We want a large deviation principle of the joint process \m{Z_t^ε = (X_t^ε - W_T, Y_t^ε)}.

	We take a sequence of stopping times \m{(τ_n)} such that \m{τ_n ↗ T_b}. Then

	\startsection [title={\m{\tilde{W}_⋅} is a Wiener process}]

		We show that \m{(\tilde{W}_t)} is a \m{(\tilde{ℱ}_t)}-martingale with quadratic variation \m{t}. Then by Lévy's Characterization of Wiener process, we obtain that \m{\tilde{W}_⋅} is a Wiener process.

		First we prove two lemmas.

		\startlemma [reference=lemma:equality-of-σalgebras]
			The σ-algebras \m{ℱ_s ∨ σ(W_T)} and \m{ℱ_s ∨ σ(W_T - W_s)} are the same.
		\stoplemma

		\startproof
			For any Borel set \m{B}, the set \m{\bcrl[W_T ∈ B] = \bcrl[(W_T - W_t) + W_t ∈ B]}.

			TODO
		\stopproof

		\startlemma [reference=lemma:conditional-expectation-of-W_t-W_s]
			For \m{0 ≤ s ≤ t ≤ T}, we have
			\startformula
				𝔼(W_t - W_s ∣ W_T - W_s) = \frac{t - s}{T - s} (W_T - W_s) .
			\stopformula
		\stoplemma

		\startproof
			We partition the interval \m{[0, T]} into \m{n = k n_0} equal parts, where \m{n_0 = \brnd[\min{\bcrl[s, t - s, T - t]}]^{-1}} and \m{k ∈ ℕ}. Let \m{n_s = s \frac{n}{T}} and \m{n_t = t \frac{n}{T}}. That is, the partition is
			\startformula
				P = \bcrl[0, \frac{T}{n}, …, \frac{n_s T}{n} = s, …, \frac{n_t T}{n} = t, …, \frac{(n - 1)T}{n}, T] .
			\stopformula

			Let \m{Δ_i W = W_{\frac{(i + 1) T}{n}} - W_{\frac{i T}{n}}}.

			Firstly, note that the \m{Δ_i W}s are independent and identically distributed from the definition of Wiener process. Now, using the linearity of conditional expectation, we have
			\startformula  \startalign
				\NC  𝔼(W_t - W_s ∣ W_T - W_s)  =  \NC  𝔼 \brnd[∑_{i = n_s}^{n_t - 1} Δ_i W ∣ ∑_{i = n_s}^{n_t - 1} Δ_i W]  \NR
				\NC  =  \NC  ∑_{i = n_s}^{n_t - 1} 𝔼 \brnd[Δ_i W ∣ ∑_{i = n_s}^{n - 1} Δ_i W]  \NR
				\NC  =  \NC  ∑_{i = n_s}^{n_t - 1} \frac{1}{n - n_s} ∑_{i = n_s}^{n - 1} 𝔼 \brnd[Δ_i W ∣ ∑_{i = n_s}^{n - 1} Δ_i W]  \NR
				\NC  =  \NC  ∑_{i = n_s}^{n_t - 1} \frac{1}{n - n_s}  𝔼 \brnd[∑_{i = n_s}^{n - 1} Δ_i W ∣ ∑_{i = n_s}^{n - 1} Δ_i W]  \NR
				\NC  =  \NC  ∑_{i = n_s}^{n_t - 1} \frac{1}{n - n_s}  ∑_{i = n_s}^{n - 1} Δ_i W  \NR
				\NC  =  \NC  ∑_{i = n_s}^{n_t - 1} \frac{1}{n - n_s}  (W_T - W_s)  \NR
				\NC  =  \NC  \frac{n_t - n_s}{n - n_s}  (W_T - W_s)  \quad  =  \quad  \frac{t - s}{T - s}  (W_T - W_s) . \NR
			\stopalign  \stopformula
		\stopproof


		\startproposition
			\m{\tilde{W}_⋅} is a \m{\tilde{ℱ}_⋅}-martingale.
		\stopproposition

		\startproof
			Let \m{0 ≤ s ≤ t ≤ T}. Then
			\startformula
				\tilde{W}_t - \tilde{W}_s
				=  (W_t - W_s) - ∫_s^t \frac{W_T - W_u}{T - u} \d u
				=  (W_t - W_s) - ∫_s^t \brnd[\frac{W_T - W_s}{T - u} - \frac{W_u - W_s}{T - u}] \d u .
			\stopformula

			Moreover, since \m{W_t - W_s} is independent of \m{ℱ_s} for every \m{t ≥ s}, using lemmas \in[lemma:equality-of-σalgebras] and \in[lemma:conditional-expectation-of-W_t-W_s], we get
			\startformula
				𝔼(W_t - W_s ∣ \tilde{ℱ}_s)
				=  𝔼 \brnd[W_t - W_s ∣ ℱ_s ∨ σ(W_T - W_s)]
				=  𝔼 \brnd[W_t - W_s ∣ W_T - W_s] = \frac{t - s}{T - s} (W_T - W_s) .
			\stopformula

			Therefore, using the fact that \m{W_T} and \m{W_s} are \m{\tilde{ℱ}_s}-measurable with conditional Fubini's theorem, we get
			\startformula  \startalign
				\NC  𝔼(\tilde{W}_t - \tilde{W}_s ∣ \tilde{ℱ}_s)
				     =  \NC  𝔼 \brnd[W_t - W_s ∣ \tilde{ℱ}_s] - ∫_s^t \brnd[\frac{W_T - W_s}{T - u} - \frac{𝔼 \brnd[W_u - W_s ∣ \tilde{ℱ}_s]}{T - u}] \d u  \NR
				\NC  =  \NC  \frac{t - s}{T - s} (W_T - W_s) - ∫_s^t \brnd[\frac{W_T - W_s}{T - u} - \frac{u - s}{T - s} \frac{W_T - W_s}{T - u}] \d u  \NR
				\NC  =  \NC  \frac{t - s}{T - s} (W_T - W_s) - ∫_s^t \frac{W_T - W_s}{T - s} \d u  \NR
				\NC  =  \NC  \frac{t - s}{T - s} (W_T - W_s) - \frac{t - s}{T - s} (W_T - W_s)  \quad  =  \quad  0 . \NR
			\stopalign  \stopformula

			Now, since \m{\tilde{W}_s} is \m{\tilde{ℱ}_s}-measurable, \m{𝔼(\tilde{W}_t ∣ \tilde{ℱ}_s) = 𝔼(\tilde{W}_t - \tilde{W}_s ∣ \tilde{ℱ}_s) + \tilde{W}_s = \tilde{W}_s}.
		\stopproof


		\startproposition
			The quadratic variation of \m{\tilde{W}_t} is \m{t}.
		\stopproposition

		% \startproof
		% 	TODO
		% \stopproof

	\stopsection

\stopchapter

\stopcomponent

% \startformula  \startalign
	
% \stopalign  \stopformula
