\startcomponent *

\product  prd-analysis

\startchapter[title={Elementary ideas}]

	\startsection [title={\m{Ïƒ}-algebras}]
		\startitemize [1, nowhite, after]
			\item  \m{ğ“˜ âŠ‚ ğ“‘ âŠ‚ \overline{ğ“‘} = ğ“› âŠ‚ 2^â„}    % TODO: Add counterexamples
			\item  \m{\abs[ğ“˜] = \abs[ğ“‘] = \abs[â„] = â„µ_{1}, \ \abs[\overline{ğ“‘}] = \abs[2^â„] = â„µ_{2}}
		\stopitemize
	\stopsection

	\startsection [title={Examples}]
		\startitemize [1, nowhite, after]
			\item  \m{\brnd[x â†¦ \frac{1}{\sqrt{x}} ğŸ™_{[0, 1]}(x)] âˆˆ L^1 âˆ– L^2}
			\item  \m{\brnd[x â†¦ \frac{1}{x} ğŸ™_{[1, âˆ)}(x)] âˆˆ L^2 âˆ– L^1}
		\stopitemize
	\stopsection

	\startsection [title={Measurability of \m{\inf, \sup, \liminf, \limsup} TODO}]
		Let \m{X_n} be a discrete-time stochastic process.
		Then \m{\bcrl[\inf X_t â‰¥ c]  =  â‹‚_t \bcrl[X_t â‰¥ c]  }
	\stopsection

	\startsection [title={Method of substitution}]
		See Folland - Real Analysis Theorem (2.43).
	\stopsection

\stopchapter


\startchapter [title={Borel--Cantelli lemmas}]

	\starttheorem[title={Borel--Cantelli 1}]
		Let \m{(E_n) âŠ‚ â„±} such that \m{âˆ‘â„™(E_n) < âˆ}. Then \m{â„™\brnd[E_n \infinitelyoften] = 0}.
	\stoptheorem
	\startproof
		Since \m{âˆ‘â„™(E_n) < âˆ}, for any fixed \m{n âˆˆ â„•}, we have
		\startformula
			â„™\brnd[E_n \infinitelyoften]  =  â„™\brnd[â‹‚_{n} â‹ƒ_{m â‰¥ n} E_m]  â‰¤  â„™\brnd[â‹ƒ_{m â‰¥ n} E_m]  â‰¤  âˆ‘_{m â‰¥ n} â„™(E_n)  â†’  0 .
		\stopformula
	\stopproof

	Counterexample of the converse of BC1: Take \m{((0, 1], Î»)} as the probability space, and \m{E_n = \brnd[0, \frac{1}{n^2}]}. Then \m{â„™\brnd[E_n \infinitelyoften] = 1}, but \m{âˆ‘â„™(E_n) < âˆ}.

	\starttheorem[title={Borel--Cantelli 2}]
		Let \m{(E_n) âŠ‚ â„±} be (mutually) independent such that \m{âˆ‘â„™(E_n) = âˆ}. Then \m{â„™\brnd[E_n \infinitelyoften] = 1}.
	\stoptheorem
	\startproof
		Since \m{â„™\brnd[{\brnd[E_n \infinitelyoften]}^âˆ] = â„™\brnd[E_n^âˆ \eventually]}, it is equivalent to prove that \m{â„™\brnd[E_n^âˆ \eventually] = 0}. Using independence and the fact that \m{1 - x < e^{-x}}, for each fixed \m{n âˆˆ â„•}, we have
		\startformula
			â„™\brnd[â‹‚_{m = n}^N E_n^âˆ]  =  âˆ_{m = n}^N â„™\brnd[E_n^âˆ]  =  âˆ_{m = n}^N \brnd[1 - â„™(E_n)]  â‰¤  âˆ_{m = n}^N e^{- â„™(E_n)}  =  e^{- âˆ‘_{m = n}^N â„™(E_n)} .
		\stopformula
		Taking \m{N â†’ âˆ}, we get \m{â„™\brnd[â‹‚_{m â‰¥ n} E_n^âˆ] â†’ 0}. Therefore
		\startformula
			â„™\brnd[E_n^âˆ \eventually]  =  â„™\brnd[â‹ƒ_n â‹‚_{m â‰¥ n} E_n^âˆ]   â‰¤  âˆ‘_n â„™\brnd[â‹‚_{m = n}^N E_n^âˆ]  =  0 .
		\stopformula
	\stopproof

\stopchapter


\startchapter [title={Modes of convergence}]

	Study this part from \goto{Robert L Wolpert - Convergence in \m{â„^d} and in metric spaces}[url(https://www2.stat.duke.edu/courses/Fall18/sta711/lec/wk-07.pdf)].
	% ToDo: Correct this diagram.
	In this diagram, the top row represents \quote{\emph{point independent}} modes of convergence and the bottom row represents the \quote{\emph{point dependent}} modes of convergence.

	\blank[line]

	\starttikzcd [row sep=huge, column sep=huge]
		unif
				\arrow[r, middlegreen]
				\arrow[d, middlegreen]
			\NC  L^âˆ
				\arrow[r, middlegreen]
				\arrow[d, middlegreen]
			\NC  L^2
				\arrow[r, middlegreen]
				\arrow[dl, slategray, swap, "(X_n âŸ‚) âˆ§ (ğ”¼ X_n = 0) âˆ§ (âˆ‘ ğ• X_n < âˆ)" description]
			\NC  L^1
				\arrow[r, middlegreen]
			\NC  â„™
				\arrow[r, middlegreen]
				\arrow[dlll, bend left, magenta, "âˆ€ \text{ subseq } âˆƒ \text{ subsubseq }" description]
				\arrow[l, bend right, darkblue, swap, "\text{u.i. âˆ¨ unif bound}"]
			\NC  w^*
				\arrow[l, bend right, swap, darkorange, "const" description]
		\NR  pt
				\arrow[r, middlegreen]
			\NC  a.s.
				\arrow[urrr, middlegreen]
				\arrow[urr, dotted, red, near end, "LDCT?" description]  \NR
	\stoptikzcd

	Legend
	\startitemize [1, nowhite, after]
		\item  \color[middlegreen]{green: automatic implication}
		\item  any other color: depends on the mentioned condition
	\stopitemize

\stopchapter


\startchapter [title={Conditioning}, reference=sec:conditioning]

	\startsection[title={In \m{L^2}, conditional expectation is a projection}]
		Let \m{(Î©, â„±, â„™)} be a probability space, \m{ğ“– âŠ† â„±} be a sub-Ïƒ-algebra, and \m{X âˆˆ L^2(â„±)} be a random variable. Let \m{Ï€_{L^2(ğ“–)}} denote the projection operator onto \m{L^2(ğ“–)}. We know that projection operators are self-adjoint. So \m{âˆ€ E âˆˆ ğ“–},
		\startformula \startalign[n=3]
			\NC  âˆ«_E ğ”¼(X âˆ£ ğ“–) \d â„™ \big|_ğ“–  \NC =  âˆ«_E X \d â„™  =  âˆ« ğŸ™_E X \d â„™  =  \inn[ğŸ™_E, X]  \NC  [\text{definitions}]  \NR
			\NC  \NC =  \inn[Ï€_{L^2(ğ“–)} ğŸ™_E, X]  \NC  [E âˆˆ ğ“– âŸ¹ ğŸ™_E âˆˆ L^2(ğ“–)]  \NR
			\NC  \NC =  \inn[ğŸ™_E, Ï€_{L^2(ğ“–)}^* X]  =  \inn[ğŸ™_E, Ï€_{L^2(ğ“–)} X]  \NC  [\text{self-adjointness}]  \NR
			\NC  \NC =  âˆ« ğŸ™_E Ï€_{L^2(ğ“–)} X \d â„™ \big|_ğ“–  =  âˆ«_E Ï€_{L^2(ğ“–)} X \d â„™ \big|_ğ“– .  \qquad  \NC  [\text{definitions}]  \NR
		\stopalign \stopformula
		Therefore, \m{ğ”¼(X âˆ£ ğ“–) = Ï€_{L^2(ğ“–)} X} a.s.

	\stopsection

	\startsection [title={Uncorrelated does not imply independence}]
		See the wikipedia entries on \goto{uncorrelated random variables}[url(https://en.wikipedia.org/wiki/Uncorrelated_random_variables)] and \goto{normally distributed and uncorrelated does not imply independent}[url(https://en.wikipedia.org/wiki/Normally_distributed_and_uncorrelated_does_not_imply_independent)].
	\stopsection

	\startsection [title={\m{Ï•_{aX + bY} = Ï•_{aX} Ï•_{bY} \ âˆ€ (a, b) âˆˆ â„^2} implies independence}]
		See \goto{MathSx:1802289}[url(https://math.stackexchange.com/questions/1802289)].
	\stopsection

\stopchapter

\stopcomponent
